workloads/Rocq/BSTProplang/Src/Impl.v
@@ -19,25 +19,26 @@ Fixpoint insert (k : nat) (v: nat) (t : Tree) :=
   match t with
   | E => T E k v E
   | T l k' v' r => 
-  (*! *)                 
+  (*! *)
+    (*!
     if k <? k' then T (insert k v l) k' v' r 
     else if k' <? k then T l k' v' (insert k v r) 
     else T l k' v r
-  (*!! insert_1  *)
-  (*!
+    *)
+  (*!! insert_1 *)
     T E k v E
-  *)
   (*!! insert_2 *)
-(*!
-  if k <? k' then T (insert k v l) k' v' r
-  else T l k' v r *)
- 
+  (*!
+    if k <? k' then T (insert k v l) k' v' r
+    else T l k' v r
+  *)
   (*!! insert_3 *)
-  
-  (*! if k <? k' then T (insert k v l) k' v' r
-  else if k' <? k then T l k' v' (insert k v r)
-  else T l k' v' r *)
- 
+  (*!
+    if k <? k' then T (insert k v l) k' v' r
+    else if k' <? k then T l k' v' (insert k v r)
+    else T l k' v' r
+  *)
+  (* !*)
   end.
 
 Fixpoint join (l: Tree) (r: Tree) :=
@@ -70,6 +71,7 @@ Fixpoint delete (k: nat) (t: Tree) :=
   else if k <? k' then T l k' v' (delete k r)
   else join l r
   *)
+  (* !*)
   end.
 
 
@@ -109,7 +111,7 @@ Fixpoint union_ (l: Tree) (r: Tree) (f: nat) :=
       T l k v (T (union_ r l' f') k' v' r')
     *)
     (*!! union_7 *)
-    (*!     
+    (*!
     | (T l k v r), (T l' k' v' r') =>
       if k =? k' then T (union_ l l' f') k v (union_ r r' f')
       else if k <? k' then T l k v (T (union_ r l' f') k' v' r')
@@ -123,6 +125,7 @@ Fixpoint union_ (l: Tree) (r: Tree) (f: nat) :=
                             (union_ r (T (above k l') k' v' r') f')
       else union_ (T l' k' v' r') (T l k v r) f' 
     *)
+    (* !*)
     end
   end
 .
