workloads/Rocq/Lib/loops/PreconditionBypassingLoop.v
@@ -1,0 +1,31 @@
+
+
+Definition runLoopBypassPreconditions (fuel : nat) (cprop : CProp ∅): G Result :=  
+  let fix runLoop'
+    (fuel : nat) 
+    (cprop : CProp ∅) 
+    (passed : nat)
+    (discards: nat)
+    : G Result :=
+    match fuel with
+    | O => ret (mkResult discards false passed [])
+    | S fuel' => 
+        res <- generate_and_run_bypassing_preconditions cprop (log2 (passed + discards)%nat);;
+        match res with
+        | Normal seed false =>
+            (* Fails *)
+            let shrunk := shrinker cprop seed in
+            let printed := printer cprop shrunk in
+            ret (mkResult discards true (passed + 1) printed)
+        | Normal _ true =>
+            (* Passes *)
+            runLoop' fuel' cprop (passed + 1)%nat discards
+        | Discard _ _ => 
+          (* Discard *)
+          runLoop' fuel' cprop passed (discards + 1)%nat
+        end
+    end in
+    runLoop' fuel cprop 0%nat 0%nat
+    .
+
+    
