workloads/Rocq/Lib/loops/TargetLoop.v
@@ -1,0 +1,76 @@
+Require Import String ZArith List Nat.
+
+From QuickChick Require Import QuickChick.
+From PropLang Require Import PropLang SeedPool.
+
+Import ListNotations.
+Import QcNotation.
+Import MonadNotation.
+
+
+Local Open Scope string.
+Local Open Scope qc_scope.
+Local Open Scope Z.
+Local Open Scope nat_scope.
+Local Open Scope prop_scope.
+
+
+Definition targetLoop
+  (fuel : nat) 
+  (cprop : CProp ∅)
+  (feedback_function: ⟦⦗cprop⦘⟧ -> Z)
+  {Pool : Type}
+  {poolType: @SeedPool (⟦⦗cprop⦘⟧) Z Pool}
+  (seeds : Pool)
+  (utility: Utility) : G Result :=
+  let fix targetLoop' 
+         (fuel : nat) 
+         (passed : nat)
+         (discards: nat)
+         {Pool : Type}
+         (seeds : Pool)
+         (poolType: @SeedPool (⟦⦗cprop⦘⟧) Z Pool)
+         (utility: Utility) : G Result :=
+        match fuel with
+        | O => ret (mkResult discards false passed [])
+        | S fuel' => 
+            let directive := sample seeds in
+            input <- generator cprop directive (log2 (passed + discards));;
+            match lift_opt_cprop cprop input with
+            | None =>
+                let seeds' := match directive with
+                            | Generate => seeds
+                            | Mutate _ => revise seeds
+                            end in
+                targetLoop' fuel' passed (discards + 1) seeds' poolType utility
+            | Some input =>
+							let '(result, feedback) := instrumented_runner cprop with_instrumentation input in
+							match result with
+							| Some false =>
+									(* Fails *)
+									let shrunk := shrinker cprop input in
+									let printed := printer cprop shrunk in
+									ret (mkResult discards true (passed + 1) printed)
+							| Some true =>
+									(* Passes *)
+									let feedback := feedback_function input in
+									match useful seeds feedback with
+									| true =>
+											let seeds' := invest (input, feedback) seeds in
+											targetLoop' fuel' (passed + 1) discards seeds' poolType utility
+									| false =>
+											let seeds' := match directive with
+																		| Generate => seeds
+																		| Mutate source => revise seeds
+																		end in
+											targetLoop' fuel' (passed + 1) discards seeds' poolType utility
+									end
+							| None =>
+									(* Discard *)
+									targetLoop' fuel' passed (discards + 1) seeds poolType utility
+							end
+						end
+        end in
+        targetLoop' fuel 0 0 seeds poolType utility.
+
+
