workloads/Rocq/Lib/seedpool/Heap.v
@@ -1,0 +1,134 @@
+
+
+Module LeftistHeap.
+
+  Inductive LTree (A : Type) : Type :=
+  | E : LTree A
+  | N : nat -> A -> LTree A -> LTree A -> LTree A.
+
+  Arguments E {A}.
+  Arguments N {A} _ _ _ _.
+
+  Definition right_spine {A : Type} (t : LTree A) : nat :=
+  match t with
+    | E => 0
+    | N r _ _ _ => r
+  end.
+
+  Inductive LeftBiased {A : Type} : LTree A -> Prop :=
+    | LeftBiased_E : LeftBiased E
+    | LeftBiased_N :
+        forall (v : A) (l r : LTree A),
+          (right_spine r <= right_spine l)%nat ->
+          LeftBiased l -> LeftBiased r ->
+            LeftBiased (N (1 + right_spine r) v l r).
+
+  Inductive Elem {A : Type} (x : A) : LTree A -> Prop :=
+    | Elem_root :
+        forall (n : nat) (l r : LTree A), Elem x (N n x l r)
+    | Elem_l :
+        forall (n : nat) (v : A) (l r : LTree A),
+          Elem x l -> Elem x (N n v l r)
+    | Elem_r :
+        forall (n : nat) (v : A) (l r : LTree A),
+          Elem x r -> Elem x (N n v l r).
+
+  Definition Heap {A F: Type} := LTree (@Seed A F).
+
+  Definition seed_in_z {A F: Type} `{Scalar F} (x: @Seed A F) : Z := scale (feedback x).
+
+  Inductive isHeap {A F: Type} `{Scalar F} : @Heap A F -> Prop :=
+    | isHeap_E : isHeap E
+    | isHeap_N :
+        forall  (n: nat) (v: Seed) (l r : Heap),
+          (forall x : @Seed A F, Elem x l -> seed_in_z v >= seed_in_z x) -> isHeap l ->
+          (forall x : @Seed A F, Elem x r -> seed_in_z v >= seed_in_z x) -> isHeap r ->
+            isHeap (N n v l r).
+
+  #[global] Hint Constructors LTree LeftBiased Elem isHeap : core.
+
+  Definition balance {A F: Type}
+    (v : @Seed A F) (l r : Heap) : Heap :=
+    if (right_spine r <=? right_spine l)%nat
+    then N (1 + right_spine r) v l r
+    else N (1 + right_spine l) v r l.
+
+  Fixpoint size {A F: Type} (t : @Heap A F) : nat :=
+  match t with
+    | E => 0
+    | N _ _ l r => 1 + size l + size r
+  end.
+
+  Definition sum_of_sizes
+    {A F: Type}
+    (p : @Heap A F * @Heap A F) : nat :=
+    size (fst p) + size (snd p).
+
+  Function merge {A F: Type} (p : @Heap A F * @Heap A F) (witness: Scalar F) {measure sum_of_sizes p} : @Heap A F :=
+  match p with
+    | (E, t2) => t2
+    | (t1, E) => t1
+    | (N _ v l r as t1, N _ v' l' r' as t2) =>
+        if ((seed_in_z v) >=? (seed_in_z v'))%Z
+        then balance v l (merge (r, t2) witness)
+        else balance v' l' (merge (t1, r') witness)
+  end.
+  Proof.
+  1-2: intros; cbn; lia.
+  Defined.
+
+  Definition empty {A F: Type} (tt: unit) : @Heap A F := E.
+
+  Definition isEmpty {A F: Type} (t : @Heap A F) : bool :=
+  match t with
+    | E => true
+    | _ => false
+  end.
+
+  Definition singleton {A F: Type} (x : @Seed A F) : Heap := N 1 x E E.
+
+  Definition insert {A F: Type} `{w: Scalar F} (x : @Seed A F) (t : Heap) : Heap :=
+  @merge A F (singleton x, t) w.
+
+  Definition findMax {A F: Type} (t : Heap) : option (@Seed A F) :=
+  match t with
+    | E => None
+    | N _ v _ _ => Some v
+  end.
+
+  Definition deleteMax {A F: Type} `{w: Scalar F} (t : Heap) : option Seed * Heap :=
+  match t with
+    | E => (None, E)
+    | N _ v l r => (Some v, @merge A F (l, r) w)
+  end.
+
+  Definition extractMax {A F: Type} `{w: Scalar F}
+  (t : Heap) : option (Seed * Heap) :=
+  match t with
+    | E => None
+    | N _ v l r => Some (v, @merge A F (l, r) w)
+  end.
+
+End LeftistHeap.
+
+#[global] Instance HeapSeedPool {A F: Type} `{Scalar F} : @SeedPool A F (@LeftistHeap.Heap A F) :=
+{| mkPool _ := LeftistHeap.empty tt;
+  invest seed pool := match seed with 
+                      | (a, f) => LeftistHeap.insert (mkSeed a f 100) pool
+                      end ;
+  revise pool :=  match LeftistHeap.extractMax pool with
+                  | None => pool
+                  | Some (seed, rest) => 
+                    let '{| input := a; feedback := f; energy := n|} := seed in
+                    if (n =? 0) then rest
+                    else LeftistHeap.insert (mkSeed a f (n - 1)) rest
+                  end ;
+  sample pool := match LeftistHeap.extractMax pool with
+                 | None => Generate
+                 | Some (seed, _) => Mutate seed
+                 end ;
+  best pool := match LeftistHeap.extractMax pool with
+               | None => None
+               | Some (seed, _) => Some seed
+               end
+|}.
