workloads/Rocq/Lib/seedpool/SeedPool.v
@@ -1,0 +1,86 @@
+Require Import String ZArith List.
+
+From QuickChick Require Import QuickChick.
+From PropLang Require Import PropLang.
+
+Import ListNotations.
+Import QcNotation.
+Import MonadNotation.
+
+Local Open Scope string.
+Local Open Scope qc_scope.
+Local Open Scope nat_scope.
+Local Open Scope Z.
+Local Open Scope prop_scope.
+
+
+Record Seed {A F: Type} := {
+  input: A;
+  feedback: F;
+  energy: Z;
+}.
+
+Definition mkSeed {A F: Type} (a: A) (f: F) (e: Z): Seed := {| input := a; feedback := f; energy := e |}.
+
+Definition Temperature := Z.
+
+Inductive Directive {A F: Type} :=
+| Generate : Directive
+| Mutate : @Seed A F -> Directive
+.
+
+#[global] Instance showDirective {A F: Type} `{Show (@Seed A F)}  : Show (@Directive A F) :=
+{|
+  show d := match d with
+            | Generate => "Generate"
+            | Mutate seed => "Mutate(" ++ show seed ++ ")"
+            end
+|}.
+
+Definition generator (cprop: CProp ∅) (directive: @Directive ⟦⦗cprop⦘⟧ Z) (size: nat) : G ⟦⟬cprop⟭⟧ :=
+  match directive with
+  | Generate => generate_cprop cprop size
+  | Mutate seed => mut_all cprop size (input seed)
+  end.
+
+Class SeedPool {A F Pool: Type} := {
+  (* Creates an empty pool. *)
+  mkPool  : unit -> Pool;
+  (* Adds a useful seed into the pool. *)
+  invest  : (A * F) -> Pool -> Pool;
+  (* Decreases the energy of a seed after a useless trial. *)
+  revise  : Pool -> Pool;
+  (* Samples the pool for an input. *)
+  sample  : Pool -> @Directive A F;
+  (* Returns the best seed in the pool. *)
+  best    : Pool -> option (@Seed A F);
+}.
+
+Class Utility {A F Pool: Type} `{SeedPool A F Pool} := {
+  (* Returns true if the feedback is interesting. *)
+  useful  : Pool -> F -> bool;
+  (* Returns a metric of how interesting the feedback is. *)
+  utility : Pool -> F -> Z;
+}.
+
+Class Scalar (A : Type) :=
+  { scale : A -> Z }.
+
+#[global] Instance ScalarZ : Scalar Z :=
+  {| scale := fun x => x |}.
+
+#[global] Instance ScalarNat : Scalar nat :=
+{| scale := fun x => Z.of_nat x |}.
+
+#[global] Instance HillClimbingUtility {A F Pool} `{SeedPool A F Pool} `{Scalar F} 
+: Utility := 
+{|
+  useful  := fun pool feedback' => match best pool with
+                                  | None => true
+                                  | Some seed => (scale feedback') >? (scale (feedback seed))
+                                  end;
+  utility := fun pool feedback' => match best pool with
+                                  | None => scale feedback'
+                                  | Some seed => scale feedback' - (scale (feedback seed))
+                                  end
+|}.
